Domain for memTaint map must be total

src/arch/x64/X64.Machine_s.fst
@@ -64,3 +64,5 @@ type observation =
   | BranchPredicate: pred:bool -> observation
   | MemAccess: addr:nat64 -> observation
   | MemAccessOffset: base:nat64 -> index:nat64 -> observation
+
+type memTaint_t = (m:Map.t int taint{Map.domain m == Set.complement Set.empty})
